translator/ml_translatorScript.sml
@@ -322,15 +322,9 @@ val Eval_Recclosure = store_thm("Eval_Recclosure",
   Eval ((name,v)::(fname,Recclosure env2 [(fname,name,body)] fname)::env2) body (b (f n))) ==>
     LOOKUP_VAR fname env (Recclosure env2 [(fname,name,body)] fname) ==>
     Eval env (Var (Short fname)) ((Eq a n --> b) f)``,
-  NTAC 2 STRIP_TAC \\ IMP_RES_TAC LOOKUP_VAR_THM
-  \\ POP_ASSUM MP_TAC \\ POP_ASSUM (K ALL_TAC) \\ POP_ASSUM MP_TAC
-  \\ FULL_SIMP_TAC std_ss [Eval_def,Arrow_def] \\ REPEAT STRIP_TAC
-  \\ POP_ASSUM MP_TAC \\ ONCE_REWRITE_TAC [evaluate'_cases]
-  \\ FULL_SIMP_TAC (srw_ss()) [AppReturns_def,Eq_def,
-       do_app_def,evaluate_closure_def]
-  \\ REPEAT STRIP_TAC \\ FULL_SIMP_TAC (srw_ss()) []
-  \\ SIMP_TAC (srw_ss()) [Once find_recfun_def,Eval_def]
-  \\ FULL_SIMP_TAC (srw_ss()) [bind_def,build_rec_env_def,FOLDR,tenv_add_tvs_def]);
+  (Eval_Recclosure_ALT |> Q.SPECL [`[(fname,name,body)]`,`fname`]
+    |> SIMP_RULE (srw_ss()) [Once find_recfun_def] |> ASSUME_TAC)
+  \\ FULL_SIMP_TAC std_ss []);
 
 val SafeVar_def = Define `SafeVar = Var`;
 
@@ -887,6 +881,39 @@ val DeclAssum_Dlet_INTRO = store_thm("DeclAssum_Dlet_INTRO",
   \\ FULL_SIMP_TAC std_ss [Eval_def] \\ REPEAT STRIP_TAC \\ RES_TAC
   \\ metis_tac [big_exp_determ', PAIR_EQ, result_11, evaluate'_empty_store_IMP])
 
+val DeclAssum_Dletrec_INTRO_ALT = store_thm("DeclAssum_Dletrec_INTRO_ALT",
+  ``!funs.
+      (!env1 env.
+        DeclAssum ds env /\
+        EVERY ( \ (P,(v,rest)).
+          LOOKUP_VAR v env1 (Recclosure env (MAP SND funs) v)) funs ==>
+        EVERY ( \ (P,(v,rest)).
+          Eval env1 (Var (Short v)) P) funs) ==>
+      !env. DeclAssum (SNOC (Dletrec (MAP SND funs)) ds) env ==>
+            EVERY ( \ (P,(v,rest)).
+              Eval env (Var (Short v)) P) funs``,
+  STRIP_TAC
+  \\ FULL_SIMP_TAC std_ss [DeclAssum_def,SNOC_APPEND,Decls_APPEND,Decls_Dletrec,
+       MAP,ALL_DISTINCT,MEM,PULL_EXISTS,build_rec_env_def,FOLDR,bind_def,
+       Eval_Var_SIMP,LOOKUP_VAR_SIMP,EVERY_MEM,FORALL_PROD]
+  \\ SIMP_TAC std_ss [Eval_def] \\ ONCE_REWRITE_TAC [evaluate'_cases]
+  \\ SIMP_TAC (srw_ss()) [] \\ REPEAT STRIP_TAC
+  \\ FULL_SIMP_TAC std_ss [PULL_FORALL,AND_IMP_INTRO]
+  \\ Q.PAT_ASSUM `!env1.bbb` MATCH_MP_TAC
+  \\ Q.LIST_EXISTS_TAC [`env2`,`s2`,`cenv2'`] \\ FULL_SIMP_TAC std_ss []
+  \\ Q.LIST_EXISTS_TAC [`p_1''`,`p_2`]
+  \\ FULL_SIMP_TAC std_ss [merge_def,emp_def,APPEND_NIL,LOOKUP_VAR_def]
+  \\ NTAC 5 STRIP_TAC
+  \\ Q.MATCH_ASSUM_RENAME_TAC `MEM (P,v,x,y) funs` []
+  \\ Q.SPEC_TAC (`Recclosure env2 (MAP SND funs)`,`recc`) \\ STRIP_TAC
+  \\ POP_ASSUM MP_TAC \\ REPEAT (POP_ASSUM (K ALL_TAC))
+  \\ Induct_on `funs` \\ FULL_SIMP_TAC std_ss [MEM,FORALL_PROD,MAP,FOLDR]
+  \\ NTAC 4 STRIP_TAC
+  \\ Cases_on `(v = p_1')` \\ FULL_SIMP_TAC std_ss []
+  \\ STRIP_TAC \\ EVAL_TAC \\ FULL_SIMP_TAC std_ss []
+  \\ REPEAT (POP_ASSUM MP_TAC)
+  \\ CONV_TAC (DEPTH_CONV ETA_CONV) \\ SIMP_TAC std_ss []);
+
 val DeclAssum_Dletrec_INTRO = store_thm("DeclAssum_Dletrec_INTRO",
   ``(!env1 env.
       DeclAssum ds env /\
@@ -894,15 +921,9 @@ val DeclAssum_Dletrec_INTRO = store_thm("DeclAssum_Dletrec_INTRO",
       Eval env1 (Var (Short v)) P) ==>
     !env. DeclAssum (SNOC (Dletrec [(v,xs,f)]) ds) env ==>
           Eval env (Var (Short v)) P``,
-  FULL_SIMP_TAC std_ss [DeclAssum_def,SNOC_APPEND,Decls_APPEND,Decls_Dletrec,
-    MAP,ALL_DISTINCT,MEM,PULL_EXISTS,build_rec_env_def,FOLDR,bind_def,
-    Eval_Var_SIMP,LOOKUP_VAR_SIMP]
-  \\ SIMP_TAC std_ss [Eval_def] \\ ONCE_REWRITE_TAC [evaluate'_cases]
-  \\ SIMP_TAC (srw_ss()) [] \\ REPEAT STRIP_TAC
-  \\ Q.PAT_ASSUM `!env1.bbb` (MP_TAC o Q.SPEC `bind v (Recclosure env2 [(v,xs,f)] v) env`)
-  \\ FULL_SIMP_TAC (srw_ss()) [LOOKUP_VAR_SIMP,lookup_def,bind_def,tenv_add_tvs_def]
-  \\ FULL_SIMP_TAC (srw_ss()) [merge_def]
-  \\ METIS_TAC []);
+  (DeclAssum_Dletrec_INTRO_ALT |> Q.SPEC `[(P,v,xs,f)]`
+    |> SIMP_RULE std_ss [EVERY_DEF,MAP] |> ASSUME_TAC)
+  \\ FULL_SIMP_TAC std_ss []);
 
 (* a few misc. lemmas that help the automation *)
 
